theories/typing/lib/mutex/mutexguard.v
@@ -255,4 +255,7 @@ Section code.
     iApply type_jump; solve_typing.
   Qed.
 
+  (* TODO:
+     Should we do try_lock?
+   *)
 End code.
